separation logic based on `option mem` instead of `mem -> Prop`

compiler/src/compiler/Softmul.v
@@ -10,23 +10,221 @@ Require Import riscv.Spec.CSRFile.
 Require Import riscv.Utility.Utility.
 Require Import riscv.Utility.StringRecords.
 Import RecordNotations. (* Warnings are spurious, COQBUG https://github.com/coq/coq/issues/13058 *)
+Require Import coqutil.Decidable.
 Require Import coqutil.Z.Lia.
 Require Import coqutil.Map.Interface.
+Require Import coqutil.Datatypes.HList.
 Require Import coqutil.Tactics.Tactics.
 Require Import riscv.Utility.runsToNonDet.
 Require Import compiler.SeparationLogic.
 Require Import compiler.Simp.
+Require Import bedrock2.Syntax.
 Require Import riscv.Platform.Run.
 Require Import riscv.Utility.Encode.
 Require Import riscv.Platform.MinimalCSRs.
 Require Import riscv.Examples.SoftmulInsts.
 Require Import riscv.Platform.MaterializeRiscvProgram.
 
+Module map. Section __.
+  Context {key value} {map : map.map key value} {ok: map.ok map}.
+  Context {key_eqb: key -> key -> bool} {key_eq_dec: EqDecider key_eqb}.
+
+  Lemma put_comm: forall k1 k2 v1 v2 m,
+      k1 <> k2 ->
+      map.put (map.put m k1 v1) k2 v2 = map.put (map.put m k2 v2) k1 v1.
+  Proof.
+    intros. apply map.map_ext. intros.
+    rewrite ?map.get_put_dec.
+    destr (key_eqb k2 k); destr (key_eqb k1 k); congruence.
+  Qed.
+End __. End map.
+
+(* maybe-map *)
+Module mmap. Section __.
+  Context {key value} {map : map.map key value} {ok: map.ok map}.
+  Context {key_eqb: key -> key -> bool} {key_eq_dec: EqDecider key_eqb}.
+
+  Definition defined(mm: option map): Prop := exists m, mm = Some m.
+
+  Definition force(mm: option map): map :=
+    match mm with
+    | Some m => m
+    | None => map.empty
+    end.
+
+  (* disjoint put *)
+  Definition dput(mm: option map)(k: key)(v: value): option map :=
+    match mm with
+    | Some m =>
+      match map.get m k with
+      | Some _ => None
+      | None => Some (map.put m k v)
+      end
+    | None => None
+    end.
+
+  (* disjoint union *)
+  Definition du(a b: option map): option map :=
+    match a, b with
+    | Some a, Some b => map.fold dput (Some a) b
+    | _, _ => None
+    end.
+
+  (* disjoint-unions *)
+  Definition dus'(l: list (option map)): option map := List.fold_right du (Some map.empty) l.
+
+  Fixpoint dus (xs : list (option map)) : option map :=
+    match xs with
+    | [x] => x
+    | x :: xs => du x (dus xs)
+    | nil => Some map.empty
+    end.
+
+  Lemma du_empty_l: forall mm, du (Some map.empty) mm = mm.
+  Proof.
+    intros. simpl. destruct mm as [m|]. 2: reflexivity.
+    eapply map.fold_spec.
+    - reflexivity.
+    - intros. subst r. simpl. rewrite H. reflexivity.
+  Qed.
+
+  Lemma du_empty_r: forall mm, du mm (Some map.empty) = mm.
+  Proof.
+    intros. unfold du. destruct mm as [m|]. 2: reflexivity.
+    apply map.fold_empty.
+  Qed.
+
+  Lemma dput_comm: forall mm k1 v1 k2 v2,
+      dput (dput mm k1 v1) k2 v2 = dput (dput mm k2 v2) k1 v1.
+  Proof.
+    intros. destruct mm as [m|]; simpl. 2: reflexivity.
+    destr (key_eqb k1 k2). {
+      subst. destr (map.get m k2). 1: reflexivity.
+      simpl. rewrite !map.get_put_same. reflexivity.
+    }
+    destr (map.get m k1); simpl.
+    + destr (map.get m k2); simpl. 1: reflexivity.
+      rewrite map.get_put_diff by assumption.
+      rewrite E0. reflexivity.
+    + rewrite map.get_put_diff by congruence.
+      destr (map.get m k2); simpl. 1: reflexivity.
+      rewrite map.get_put_diff by assumption.
+      rewrite E0.
+      f_equal.
+      apply map.put_comm.
+      assumption.
+  Qed.
+
+  Lemma fold_dput_comm: forall p q, map.fold dput (Some p) q = map.fold dput (Some q) p.
+  Proof.
+    intros. eapply map.fold_spec.
+    - symmetry. clear q.
+      eapply map.fold_spec.
+      + reflexivity.
+      + intros. subst r. simpl. rewrite H. reflexivity.
+    - intros. subst. rewrite <- map.fold_comm.
+      + f_equal. simpl. rewrite H. reflexivity.
+      + intros. apply dput_comm.
+  Qed.
+
+  Lemma du_comm: forall p q, du p q = du q p.
+  Proof.
+    intros. unfold du. destruct p; destruct q; try reflexivity.
+    apply fold_dput_comm.
+  Qed.
+
+(*
+  Lemma fold_dput_assoc: forall p q r,
+      map.fold dput (map.fold dput (Some p) q) r = du (Some p) (map.fold dput (Some q) r).
+  Proof.
+    simpl.
+*)
+
+  Lemma du_assoc: forall p q r, du (du p q) r = du p (du q r).
+  Proof.
+    intros. unfold du.
+    destruct p as [p|]. 2: reflexivity.
+    destruct q as [q|]. 2: reflexivity.
+    destruct r as [r|]. 2: destruct (map.fold dput (Some p) q); reflexivity.
+    rewrite (fold_dput_comm q r).
+    eapply map.fold_two_spec with (P := fun m fold1 fold2 =>
+      match fold1 with
+      | Some a => map.fold dput (Some a) r
+      | None => None
+      end =
+      match fold2 with
+      | Some b => map.fold dput (Some p) b
+      | None => None
+      end).
+    1: reflexivity.
+    intros.
+
+(*
+    destr (map.fold dput (Some q) r); destr (map.fold dput (Some p) q).
+    - rewrite (fold_dput_comm p r0). rewrite <- E.
+      admit.
+    - rewrite fold_dput_comm. rewrite <- E. simpl.
+
+    - rewrite <- E0. rewrite (fold_dput_comm p r0). rewrite <- E.
+      rewrite (fold_dput_comm q).
+    -
+ *)
+  Admitted.
+
+  Lemma dus'_dus: forall xs, dus' xs = dus xs.
+  Proof.
+    induction xs; [reflexivity|].
+    cbn -[du]. destruct xs.
+    - cbn -[du]. apply du_empty_r.
+    - cbn [dus' fold_right]. unfold dus' in *. cbn [fold_right] in IHxs.
+      rewrite IHxs.
+      reflexivity.
+  Qed.
+
+  Lemma dus_cons: forall (P: option map) (Ps: list (option map)),
+      dus (P :: Ps) = du P (dus Ps).
+  Proof. intros. rewrite <-! dus'_dus. reflexivity. Qed.
+
+  Lemma dus_app: forall Ps Qs : list (option map),
+      dus (Ps ++ Qs) = du (dus Ps) (dus Qs).
+  Proof.
+    induction Ps; intros.
+    - cbn -[du]. simpl. symmetry. apply du_empty_l.
+    - rewrite <- List.app_comm_cons. rewrite !dus_cons. rewrite IHPs.
+      symmetry. apply du_assoc.
+  Qed.
+
+End __. End mmap.
+
+
+Module Tree.
+  Inductive t(A: Type): Type :=
+  | Leaf(a: A)
+  | Node(left right: t A).
+  Arguments Leaf {A} _.
+  Arguments Node {A} _ _.
+  Section Interp.
+    Context {A B: Type}.
+    Context (interp_Leaf: A -> B).
+    Context (interp_Node: B -> B -> B).
+    Fixpoint interp(t: t A): B :=
+      match t with
+      | Leaf a => interp_Leaf a
+      | Node t1 t2 => interp_Node (interp t1) (interp t2)
+      end.
+  End Interp.
+
+  Definition flatten{A: Type}: t A -> list A := interp (fun a => cons a nil) (@app A).
+End Tree.
+
+
 Section Riscv.
   Context {word: Word.Interface.word 32}.
   Context {word_ok: word.ok word}.
   Context {mem: map.map word byte}.
+  Context {mem_ok: map.ok mem}.
   Context {registers: map.map Z word}.
+  Context {registers_ok: map.ok registers}.
 
   (* RISC-V Monad *)
   Local Notation M := (free riscv_primitive primitive_result).
@@ -53,7 +251,7 @@ Section Riscv.
       eauto using weaken_run_primitive.
   Qed.
 
-  Lemma invert_fetch: forall initial post k,
+  Lemma invert_fetch0: forall initial post k,
       mcomp_sat (pc <- Machine.getPC; i <- Machine.loadWord Fetch pc; k i)
         initial post ->
       exists w, load_bytes 4 initial#"mem" initial#"pc" = Some w /\
@@ -64,7 +262,91 @@ Section Riscv.
     simp. eauto.
   Qed.
 
-  Lemma build_fetch: forall (initial: State) post k w,
+  Notation "a \*/ b" := (mmap.du a b) (at level 34, left associativity).
+
+  Definition tree_to_du: Tree.t (option mem) -> option mem := Tree.interp id mmap.du.
+
+  Lemma dus_flatten: forall t: Tree.t (option mem),
+      mmap.dus (Tree.flatten t) = tree_to_du t.
+  Proof.
+    induction t; [reflexivity|].
+    simpl. rewrite mmap.dus_app. rewrite IHt1, IHt2. reflexivity.
+  Qed.
+
+  Lemma tree_to_du_eq_of_flatten_eq: forall LHS RHS : Tree.t (option mem),
+      mmap.dus (Tree.flatten LHS) = mmap.dus (Tree.flatten RHS) ->
+      tree_to_du LHS = tree_to_du RHS.
+  Proof. intros. rewrite! dus_flatten in H. exact H. Qed.
+
+  Ltac reify e :=
+    lazymatch e with
+    | @mmap.du ?key ?value ?map ?a ?b =>
+      let a := reify a in
+      let b := reify b in
+      uconstr:(@Tree.Node (option (@map.rep key value map)) a b)
+    | ?a => uconstr:(Tree.Leaf a)
+    end.
+
+  Ltac reify_goal :=
+    lazymatch goal with
+    | |- @eq (option (@map.rep _ _ _)) ?LHS ?RHS =>
+      let LHS := reify LHS in
+      let RHS := reify RHS in
+      change (tree_to_du LHS = tree_to_du RHS);
+      eapply tree_to_du_eq_of_flatten_eq
+    end;
+    cbn [Tree.flatten Tree.interp app].
+
+  Section cancel_lemmas.
+    Let nth n xs := hd (@None mem) (skipn n xs).
+    Let remove_nth n (xs : list (option mem)) := firstn n xs ++ tl (skipn n xs).
+
+    Lemma cancel_at: forall (i j: nat) (xs ys: list (option mem)),
+        nth i xs = nth j ys ->
+        mmap.dus (remove_nth i xs) = mmap.dus (remove_nth j ys) ->
+        mmap.dus xs = mmap.dus ys.
+    Proof.
+    Admitted.
+  End cancel_lemmas.
+
+  Ltac cancel_at i j :=
+    lazymatch goal with
+    | |- mmap.dus ?LHS = mmap.dus ?RHS =>
+      simple refine (cancel_at i j LHS RHS _ _);
+      cbn [firstn skipn List.app hd tl]
+    end.
+
+  Definition bytes(addr: word){n: nat}(bs: tuple byte n): option mem :=
+    Some (map.of_tuple (Memory.footprint addr n) bs).
+
+  Definition array{T: Type}(elem: word -> T -> option mem)(size: word): word -> list T -> option mem :=
+    fix rec addr ls :=
+      match ls with
+      | [] => Some map.empty
+      | e :: es => elem addr e \*/ rec (word.add addr size) es
+      end.
+
+  Definition one(sz: Syntax.access_size.access_size)(addr value: word): option mem :=
+    bytes addr (LittleEndian.split (@Memory.bytes_per width sz) (word.unsigned value)).
+
+  Definition word_array: word -> list word -> option mem :=
+    array (one access_size.word) (word.of_Z bytes_per_word).
+
+  Definition instr(addr: word)(inst: Instruction): option mem :=
+    one access_size.four addr (word.of_Z (encode inst)).
+
+  Definition program(addr: word)(prog: list Instruction): option mem :=
+    array instr (word.of_Z 4) addr prog.
+
+  Lemma invert_fetch: forall initial post k,
+      mcomp_sat (pc <- Machine.getPC; i <- Machine.loadWord Fetch pc; k i) initial post ->
+      exists w R, R \*/ bytes initial#"pc" w = Some initial#"mem" /\
+                  mcomp_sat (k w) initial post.
+  Proof.
+    intros. apply invert_fetch0 in H. simp.
+  Admitted.
+
+  Lemma build_fetch0: forall (initial: State) post k w,
       load_bytes 4 initial#"mem" initial#"pc" = Some w ->
       mcomp_sat (k w) initial post ->
       mcomp_sat (pc <- Machine.getPC; i <- Machine.loadWord Fetch pc; k i) initial post.
@@ -72,6 +354,14 @@ Section Riscv.
     intros. unfold mcomp_sat in *. cbn -[HList.tuple load_bytes].
     unfold load. simpl in *. rewrite H. assumption.
   Qed.
+
+  Lemma build_fetch: forall (initial: State) post k w R,
+      mcomp_sat (k w) initial post ->
+      R \*/ bytes initial#"pc" w = Some initial#"mem" ->
+      mcomp_sat (pc <- Machine.getPC; i <- Machine.loadWord Fetch pc; k i) initial post.
+  Proof.
+    intros. eapply build_fetch0. 2: eassumption.
+  Admitted.
 
   Lemma decode_verify_iset: forall iset i, verify_iset (decode iset i) iset.
   Proof.
@@ -103,8 +393,8 @@ Section Riscv.
       map.get r2#"csrs" CSRField.MTVecBase = Some mtvec_base /\
       map.get r2#"csrs" CSRField.MScratch = Some mscratch /\
       List.length stacktrash = 32%nat /\
-      (eq r1#"mem" * word_array (word.of_Z mscratch) stacktrash *
-       program RV32I (word.of_Z (mtvec_base * 4)) handler_insts)%sep r2#"mem".
+      Some r1#"mem" \*/ word_array (word.of_Z mscratch) stacktrash \*/
+      program (word.of_Z (mtvec_base * 4)) handler_insts = Some r2#"mem".
 
   Ltac paramrecords :=
     change (@Utility.word Words32) with word in *;
@@ -153,12 +443,8 @@ Section Riscv.
     unfold related in H|-*.
     simp.
     destruct a; cbn [run_primitive] in *.
-    - exists initialH.
-      intuition (congruence || eauto 10).
-      replace initialL#"regs" with initialH#"regs" by congruence.
-      assumption.
-    - eexists. ssplit; cycle -1. 1: eassumption. all: record.simp; try congruence. 2: eauto 10.
-      destruct_one_match; congruence.
+    - exists initialH. intuition (congruence || eauto 10).
+    - exists initialH(#"regs" := setReg initialH#"regs" z r). record.simp. intuition (congruence || eauto 10).
     - eapply load_preserves_related; eauto.
     - eapply load_preserves_related; eauto.
     - eapply load_preserves_related; eauto.
@@ -216,28 +502,56 @@ Section Riscv.
       apply runsToDone. eauto.
     }
     unfold run1 in H |- *.
-    pose proof H2 as R.
+    pose proof H2 as Rel.
     unfold related in H2.
     eapply invert_fetch in H. simp.
-    pose proof (decode_verify_iset RV32IM (LittleEndian.combine 4 w)) as V.
     rename initial into initialH.
+    rewrite <- Hp0 in H2p5p3.
+    pose proof (decode_verify_iset RV32IM (LittleEndian.combine 4 w)) as V.
     destruct (decode RV32IM (LittleEndian.combine 4 w)) as
         [inst|inst|inst|inst|inst|inst|inst|inst|inst|inst] eqn: E;
-      cbn in V; try intuition congruence.
+      cbn in V; try (intuition congruence); clear V.
     - (* IInstruction *)
       eapply runsToStep with (midset0 := fun midL => exists midH, related midH midL /\ midset midH).
-      + eapply build_fetch with (w := w). {
-          case TODO. (* separation logic *)
+      + eapply build_fetch with (w := w). 2: {
+          etransitivity. 2: exact H2p5p3.
+          reify_goal.
+          cancel_at 1%nat 1%nat. 1: congruence.
+          cbn [mmap.dus].
+          reflexivity.
         }
         apply decode_I_to_IM in E. rewrite E.
         eapply mcomp_sat_preserves_related; eassumption.
       + intros midL. intros. simp. eapply H1; eassumption.
     - (* MInstruction *)
-      case TODO.
+      destruct inst.
+      + (* Mul *)
+        cbn in Hp1.
+        case TODO.
+      + (* Mulh *)
+        case TODO.
+      + (* Mulhsu *)
+        case TODO.
+      + (* Mulhu *)
+        case TODO.
+      + (* Div *)
+        case TODO.
+      + (* Divu *)
+        case TODO.
+      + (* Rem *)
+        case TODO.
+      + (* Remu *)
+        case TODO.
+      + (* InvalidM *)
+        case TODO.
     - (* CSRInstruction *)
       eapply runsToStep with (midset0 := fun midL => exists midH, related midH midL /\ midset midH).
-      + eapply build_fetch with (w := w). {
-          case TODO. (* separation logic *)
+      + eapply build_fetch with (w := w). 2: {
+          etransitivity. 2: exact H2p5p3.
+          reify_goal.
+          cancel_at 1%nat 1%nat. 1: congruence.
+          cbn [mmap.dus].
+          reflexivity.
         }
         apply decode_CSR_to_IM in E. rewrite E.
         (* lower Hr *)
